README.md
@@ -132,7 +132,7 @@ opam pin add coq-library-undecidability.dev+8.15 "https://github.com/uds-psl/coq
 
 ### Manual installation
 
-You need `Coq 8.15` built on OCAML `>= 4.07.1`, the [Smpl](https://github.com/uds-psl/smpl) package, the [Equations](https://mattam82.github.io/Coq-Equations/) package, and the [MetaCoq](https://metacoq.github.io/metacoq/) package for Coq. If you are using opam 2 you can use the following commands to install the dependencies on a new switch:
+You need `Coq 8.15` built on OCAML `>= 4.07.1` and the [MetaCoq](https://metacoq.github.io/metacoq/) package for Coq. If you are using opam 2 you can use the following commands to install the dependencies on a new switch:
 
 ```
 opam switch create coq-library-undecidability 4.07.1+flambda
